

This exercise looks into the relationship between
clauses and implication sentences.<br>

1.  Show that the clause $(\lnot P_1 \lor \cdots \lor \lnot P_m \lor Q)$
    is logically equivalent to the implication sentence
    $(P_1 \land \cdots \land P_m) {\;{\Rightarrow}\;}Q$.<br>

2.  Show that every clause (regardless of the number of
    positive literals) can be written in the form
    $(P_1 \land \cdots \land P_m) {\;{\Rightarrow}\;}(Q_1 \lor \cdots \lor Q_n)$,
    where the $P$s and $Q$s are proposition symbols. A knowledge base
    consisting of such sentences is in implicative normal form or <b>Kowalski
    form</b> @Kowalski:1979.<br>

3.  Write down the full resolution rule for sentences in implicative
    normal form.<br>
